prefix dce: <http://purl.org/dc/elements/1.1/>
prefix dct: <http://purl.org/dc/terms/>
prefix foaf: <http://xmlns.com/foaf/0.1/>
prefix owl: <http://www.w3.org/2002/07/owl#>
prefix rdf: <http://www.w3.org/1999/02/22-rdf-syntax-ns#>
prefix rdfs: <http://www.w3.org/2000/01/rdf-schema#>
prefix reco: <http://purl.org/reco#>
prefix xsd: <http://www.w3.org/2001/XMLSchema#>

reco:
  dce:contributor "Carlos Ruiz (iSOCO S.A.)", "Diego Berrueta (Fundación CTIC)", "Emilio Rubiera (Fundación CTIC)";
  dce:creator "Iván Mínguez (Fundación CTIC)", "Luis Polo (Fundación CTIC)";
  dce:date "August, 2011"@en;
  dce:description "The RECO ontology defines the vocabulary for representing prefereces-as-constraints and preferences-as-ratings as RDF graphs. This lightweight vocabulary provides domain-independent means to describe user profiles in a coherent and context-aware way. RECO has been designed as an extension of both Friend-Of-A-Friend (FOAF) and Who Am I! (WAI) ontologies."@en;
  dce:rights "Copyright by Fundación CTIC";
  dce:title "RECommendations Ontology"@en;
  dct:license <http://creativecommons.org/licenses/by-sa/3.0/>;
  a owl:Ontology;
  rdfs:isDefinedBy "http://purl.org/reco#reco.owl"^^xsd:anyURI;
  owl:priorVersion <http://ontologies.ezweb.morfeo-project.org/reco/spec/>.

reco:Demand
  a owl:Class;
  rdfs:comment "Groups of preferences representing users' requests at a given context or situation."@en;
  rdfs:label "Demand"@en;
  rdfs:subClassOf owl:Thing.

reco:Filter
  a owl:Class;
  rdfs:comment "A datatype constraint based on boolean operators."@en;
  rdfs:label "Filter"@en.

reco:Operator
  a owl:Class;
  rdfs:comment "Boolean operations on data values: string comparisons, numerical intervales and (in)equality. Operators are reused from the X-path specification to ensure interoperability."@en;
  rdfs:label "Operator"@en.

reco:Pattern
  a owl:Class;
  rdfs:comment """Patterns are reifications of constraints, which are conditions about the desired or preferred attributes of the resources. A constraint ranges over a set of individuals. RECO considers several kind of constraint expressions: (1) conjunction of constraints: "music from the sixties"; (2) disjunction of constraints: "music or films"; (3) composition of constraints: "cars with powerful engines"; (4) datatype constraints based on boolean operators: "released before 1980"."""@en;
  rdfs:label "Pattern"@en.

reco:Preference
  a owl:Class;
  rdfs:comment "A preference is a qualitative description of the desired attributes that resources must ideally satisfy in order to be of interest for a user. A preference is described by a set of constraints."@en;
  rdfs:label "Preference"@en;
  rdfs:subClassOf owl:Thing.

reco:Rating
  a owl:Class;
  rdfs:comment """A rating is a quantitative measurement of the "appealingness" of a particular item to a user."""@en;
  rdfs:label "Rating"@en.

reco:about
  a owl:FunctionalProperty, owl:ObjectProperty;
  rdfs:comment "A property that relates a preference with its main pattern."@en;
  rdfs:domain reco:Preference;
  rdfs:label "About"@en;
  rdfs:range reco:Pattern.

reco:assignedBy
  a owl:ObjectProperty;
  rdfs:comment "This property relates a rating with the person having carried out it."@en;
  rdfs:domain reco:Rating;
  rdfs:label "Assigned by"@en.

reco:excludedPreference
  a owl:ObjectProperty;
  rdfs:comment "This property relates a demand with a particular preference P. The items that fulfill the constraints of P are excluded from the set of results calculated for this demand."@en;
  rdfs:domain reco:Demand;
  rdfs:label "Excluded Preference"@en;
  rdfs:range reco:Preference;
  rdfs:subPropertyOf reco:preference.

reco:filter
  a owl:ObjectProperty;
  rdfs:comment """A property that relates a pattern with a constraint of the value of a datatype property. For instance, "less than 180 cms height" or "released before 1980"."""@en;
  rdfs:domain reco:Pattern;
  rdfs:label "Filter"@en;
  rdfs:range reco:Filter.

reco:holds
  a owl:ObjectProperty;
  rdfs:comment "This property relates a person with a preference."@en;
  rdfs:label "Holds"@en;
  rdfs:range reco:Preference.

reco:operator
  a owl:FunctionalProperty, owl:ObjectProperty;
  rdfs:comment "A property that relates a filter to the operator restraining the value of a datatype property."@en;
  rdfs:domain reco:Filter;
  rdfs:label "Operator"@en;
  rdfs:range reco:Operator.

reco:optionalPreference
  a owl:ObjectProperty;
  rdfs:comment "This property relates a demand to a preference P. The items that fulfill the constraints of P increase or decline their utility value according to the utility of P."@en;
  rdfs:domain reco:Demand;
  rdfs:label "Optional Preference"@en;
  rdfs:range reco:Preference;
  rdfs:subPropertyOf reco:preference.

reco:preference
  a owl:ObjectProperty;
  rdfs:comment "This property relates a demand with the set of preferences that defines its matchmaking conditions. "@en;
  rdfs:domain reco:Demand;
  rdfs:label "Preference"@en;
  rdfs:range reco:Preference.

reco:rates
  a owl:ObjectProperty;
  rdfs:comment "This property relates a rating with the resource assessed. Notice that this property has an open range (rdfs:Resource), therefore ratings can be applied to anything, including preferences themselves."@en;
  rdfs:domain reco:Rating;
  rdfs:label "Rates"@en.

reco:requiredPreference
  a owl:ObjectProperty;
  rdfs:comment "This property relates a demand with a preference P. The items fulfilling the constraints of P must be included in the final set of results for this demand."@en;
  rdfs:domain reco:Demand;
  rdfs:label "Required Preference"@en;
  rdfs:range reco:Preference;
  rdfs:subPropertyOf reco:preference.

reco:union
  a owl:ObjectProperty;
  rdfs:comment "A property which reifies a disjunction of constraints."@en;
  rdfs:domain reco:Pattern;
  rdfs:label "Union composition"@en;
  rdfs:range reco:Filter.

reco:utility
  a owl:DatatypeProperty;
  rdfs:comment "This property captures the utility value of a rating. The utility in RECO is measured in the real interval [-1,1]. In practice, other discrete scales can be also used to measure users' opinions on resources, such as the Likert scale. "@en;
  rdfs:domain reco:Preference;
  rdfs:label "Utility"@en;
  rdfs:range xsd:float.
